
\begin{equation}
LMSDM(a,b) = (0.4\times L(a,b)^3+0.4\times C(a,b)^3+0.2\times S(a,b)^3)^{\frac{1}{3}}
\end{equation}

\begin{equation}
 L(a,b) = \frac{||\mu_a-\mu_b||}{max(\mu_a, \mu_b)}\\
 C(a,b) = \frac{||\sigma_a-\sigma_b||}{max(\sigma_a, \sigma_b)}\\
 S(a,b) = \frac{||\sigma_a\sigma_b -\sigma_{ab}||}{\sigma_a\sigma_b}
\end{equation}

\begin{equation}
MSDM(A,B) = (\frac{1}{n_w} \sum_{j=1}^{n_w}{LMSDM(a_j,b_j)^3})^{\frac{1}{3}}
\end{equation}
\begin{equation}
LD^h(v) = 0.4\times L^h(a,b)+0.4\times C^h(a,b)+0.2\times S^h(a,b)
\end{equation}
\begin{equation}
MLD(v) = \frac{\sum_{i=1}^n{LD^{h_i}(v)}}{n}
\end{equation}
\begin{equation}
GDM(A,B) = (\frac{1}{n_A} \sum_{j=1}^{n_A}{MLD(v)^3})^{\frac{1}{3}}
\end{equation}